Factor out generic semantics helpers
Non-atomic operation combinators and dynamically-typed maps.

src/Database/DataStructures.v
@@ -6,6 +6,7 @@ From stdpp Require Import fin_maps.
 From RecoveryRefinement Require Import Helpers.MachinePrimitives.
 From RecoveryRefinement Require Import Spec.Proc.
 From RecoveryRefinement Require Import Spec.InjectOp.
+From RecoveryRefinement Require Import Spec.SemanticsHelpers.
 From RecoveryRefinement Require Import Helpers.RelationAlgebra.
 From RecoveryRefinement Require Import Helpers.GoModel.
 
@@ -118,22 +119,6 @@ Module Var.
 End Var.
 
 Instance var_eqdec : EqualDec Var.t := _.
-
-(* modeling non-atomic operations as pairs of begin/end ops *)
-Inductive NonAtomicArgs T :=
-| FinishArgs (args:T)
-| Begin.
-Arguments Begin {T}.
-(* NOTE: this does not allow dependent return values *)
-Definition retT T (args:NonAtomicArgs T) T' : Type := if args then T' else unit.
-
-(* nonAtomicOp takes an operation partially applied to some key identifying
-  the object (assuming the operation does separate over some resources, such as
-  addresses or references) *)
-Definition nonAtomicOp {Op ArgT T}
-           (op: forall (args:NonAtomicArgs ArgT), Op (retT args T))
-  : ArgT -> proc Op T :=
-  fun args => Bind (Call (op Begin)) (fun _ => Call (op (FinishArgs args))).
 
 Inductive LockMode := Reader | Writer.
 
@@ -287,20 +272,6 @@ Module Data.
 
   End OpWrappers.
 
-  (* this is represented as an inductive rather than a combination of ObjΣ and a
-  boolean state to make misuse harder (there's no reasonable way to use the
-  state without knowing the status) *)
-  Inductive NonAtomicState ObjΣ : Type :=
-  | Clean (s:ObjΣ)
-  | Dirty (s:ObjΣ).
-
-  Record DynMap A (Ref: A -> Type) (Model: A -> Type) :=
-    { dynMap : sigT Ref -> option (sigT Model);
-      dynMap_wf : forall T v, match dynMap (existT T v) with
-                         | Some (existT T' _) => T' = T
-                         | None => True
-                         end; }.
-
   Definition hashtableM V := gmap.gmap uint64 V.
 
   Inductive LockStatus := Locked | ReadLocked (num:nat) | Unlocked.
@@ -320,25 +291,6 @@ Module Data.
                             <*> hashtables
                             <*> locks)%set.
 
-  Module OptionNotations.
-    Delimit Scope option_monad with opt.
-    Notation "'Some!' x <- a ; f" :=
-      (match a with
-       | Some x => f
-       | _ => None
-       end)
-        (right associativity, at level 70, x pattern) : option_monad.
-
-    Notation "'left!' H <- a ; f" :=
-      (match a with
-       | left H => f
-       | right _ => None
-       end)
-        (right associativity, at level 60, f at level 200) : option_monad.
-
-    Notation "'ret!' a" := (Some a) (at level 60) : option_monad.
-  End OptionNotations.
-
   Import EqualDecNotation.
   Import OptionNotations.
   Local Open Scope option_monad.
@@ -353,29 +305,6 @@ Module Data.
   Definition upd_locks (r:LockRef) (v:LockStatus) (ls: LockRef -> option LockStatus) : LockRef -> option LockStatus :=
     fun r' => if r == r' then Some v else ls r'.
 
-  Definition getDyn A (Ref Model: A -> Type)
-             (m: DynMap Ref Model) a (r: Ref a) : option (Model a).
-  Proof.
-    pose proof (m.(dynMap_wf) _ r).
-    destruct (m.(dynMap) (existT a r)); [ apply Some | exact None ].
-    destruct s.
-    exact (rew H in m0).
-  Defined.
-
-  Arguments getDyn {A Ref Model} m {a} r.
-
-  Definition updDyn A (Ref Model: A -> Type) {dec: EqualDec (sigT Ref)}
-             a (v: Ref a) (x: Model a) (m: DynMap Ref Model) : DynMap Ref Model.
-  Proof.
-    refine {| dynMap := fun r => if r == existT a v then ret! existT a x else m.(dynMap) r |}.
-    intros.
-    destruct (existT _ v0 == existT _ v).
-    - inversion e; auto.
-    - apply (m.(dynMap_wf) _ v0).
-  Defined.
-
-  Arguments updDyn {A Ref Model dec a} v x m.
-
   Definition alter_map V (m: hashtableM V)
              (k:uint64) (f: option V -> option V) : hashtableM V :=
     partial_alter f k m.
@@ -383,32 +312,6 @@ Module Data.
   Close Scope option_monad.
 
   Import RelationNotations.
-
-  Definition readClean {State} ObjΣ (s: NonAtomicState ObjΣ) : relation State State ObjΣ :=
-    match s with
-    | Clean s => pure s
-    | Dirty _ => error
-    end.
-
-  Definition readDirty {State} ObjΣ (s: NonAtomicState ObjΣ) : relation State State ObjΣ :=
-    match s with
-    | Clean _ => error
-    | Dirty s  => pure s
-    end.
-
-  Definition nonAtomicStep
-             {ArgT} (args: NonAtomicArgs ArgT) {T} (* the operation *)
-             {ObjΣ} (obj_s: NonAtomicState ObjΣ)
-             {State}
-             (mkDirty: ObjΣ -> relation State State unit)
-             (opStep: ObjΣ -> ArgT -> relation State State T)
-    : relation State State (retT args T) :=
-    match args with
-    | Begin => s <- readClean obj_s;
-                mkDirty s
-    | FinishArgs x => s <- readDirty obj_s;
-                       opStep s x
-    end.
 
   (* returns [Some s'] when the lock should be acquired to status s', and None
   if the lock would block *)
@@ -526,11 +429,6 @@ Module Data.
   Definition vars0 (v:Var.t) : Var.ty v :=
     match v with
     end.
-
-  Global Instance empty_dynmap A Ref Model : Empty (@DynMap A Ref Model).
-  refine {| dynMap := fun _ => None; |}.
-  intros; auto.
-  Defined.
 
   Instance empty_state : Empty State.
   refine {| vars := vars0 ;
