src/Spec/SemanticsHelpers.v
@@ -1,0 +1,120 @@
+From Classes Require Import EqualDec.
+From stdpp Require Import base.
+
+From RecoveryRefinement Require Import Helpers.RelationAlgebra.
+From RecoveryRefinement Require Import Spec.Proc.
+
+Set Implicit Arguments.
+
+Arguments existT {A P} _ _.
+Import EqNotations.
+
+Import RelationNotations.
+
+(* modeling non-atomic operations as pairs of begin/end ops *)
+Inductive NonAtomicArgs T :=
+| FinishArgs (args:T)
+| Begin.
+Arguments Begin {T}.
+(* NOTE: this does not allow dependent return values *)
+Definition retT T (args:NonAtomicArgs T) T' : Type := if args then T' else unit.
+
+(* nonAtomicOp takes an operation partially applied to some key identifying
+  the object (assuming the operation does separate over some resources, such as
+  addresses or references) *)
+Definition nonAtomicOp {Op ArgT T}
+           (op: forall (args:NonAtomicArgs ArgT), Op (retT args T))
+  : ArgT -> proc Op T :=
+  fun args => Bind (Call (op Begin)) (fun _ => Call (op (FinishArgs args))).
+
+
+(* this is represented as an inductive rather than a combination of ObjΣ and a
+  boolean state to make misuse harder (there's no reasonable way to use the
+  state without knowing the status) *)
+Inductive NonAtomicState ObjΣ : Type :=
+| Clean (s:ObjΣ)
+| Dirty (s:ObjΣ).
+
+Definition readClean {State} ObjΣ (s: NonAtomicState ObjΣ) : relation State State ObjΣ :=
+  match s with
+  | Clean s => pure s
+  | Dirty _ => error
+  end.
+
+Definition readDirty {State} ObjΣ (s: NonAtomicState ObjΣ) : relation State State ObjΣ :=
+  match s with
+  | Clean _ => error
+  | Dirty s  => pure s
+  end.
+
+Definition nonAtomicStep
+           {ArgT} (args: NonAtomicArgs ArgT) {T} (* the operation *)
+           {ObjΣ} (obj_s: NonAtomicState ObjΣ)
+           {State}
+           (mkDirty: ObjΣ -> relation State State unit)
+           (opStep: ObjΣ -> ArgT -> relation State State T)
+  : relation State State (retT args T) :=
+  match args with
+  | Begin => s <- readClean obj_s;
+              mkDirty s
+  | FinishArgs x => s <- readDirty obj_s;
+                     opStep s x
+  end.
+
+Record DynMap A (Ref: A -> Type) (Model: A -> Type) :=
+  { dynMap : sigT Ref -> option (sigT Model);
+    dynMap_wf : forall T v, match dynMap (existT T v) with
+                       | Some (existT T' _) => T' = T
+                       | None => True
+                       end; }.
+
+Module OptionNotations.
+  Delimit Scope option_monad with opt.
+  Notation "'Some!' x <- a ; f" :=
+    (match a with
+     | Some x => f
+     | _ => None
+     end)
+      (right associativity, at level 70, x pattern) : option_monad.
+
+  Notation "'left!' H <- a ; f" :=
+    (match a with
+     | left H => f
+     | right _ => None
+     end)
+      (right associativity, at level 60, f at level 200) : option_monad.
+
+  Notation "'ret!' a" := (Some a) (at level 60) : option_monad.
+End OptionNotations.
+
+Import EqualDecNotation.
+Import OptionNotations.
+Local Open Scope option_monad.
+
+Definition getDyn A (Ref Model: A -> Type)
+           (m: DynMap Ref Model) a (r: Ref a) : option (Model a).
+Proof.
+  pose proof (m.(dynMap_wf) _ r).
+  destruct (m.(dynMap) (existT a r)); [ apply Some | exact None ].
+  destruct s.
+  exact (rew H in m0).
+Defined.
+
+Arguments getDyn {A Ref Model} m {a} r.
+
+Definition updDyn A (Ref Model: A -> Type) {dec: EqualDec (sigT Ref)}
+           a (v: Ref a) (x: Model a) (m: DynMap Ref Model) : DynMap Ref Model.
+Proof.
+  refine {| dynMap := fun r => if r == existT a v then ret! existT a x else m.(dynMap) r |}.
+  intros.
+  destruct (existT _ v0 == existT _ v).
+  - inversion e; auto.
+  - apply (m.(dynMap_wf) _ v0).
+Defined.
+
+Arguments updDyn {A Ref Model dec a} v x m.
+
+Instance empty_dynmap A Ref Model : Empty (@DynMap A Ref Model).
+refine {| dynMap := fun _ => None; |}.
+intros; auto.
+Defined.
